checker/coq/log.v
@@ -1,0 +1,145 @@
+(* Types & code for proof logs. *)
+Require Import ZArith.
+Require Import prim.
+Require Import sol.
+Require Import bounds.
+Require Import domain.
+Require Import model.
+Require Import map.
+Require Import resolution.
+Module ZMapProperties := FMapFacts.WProperties(ZMaps).
+
+Definition clause_map := zmap clause.
+Definition cst_map := zmap cst.
+
+Inductive step :=
+  | Intro : Z -> clause -> step
+  | Hint : Z -> step
+  | Del : Z -> step
+  | Resolve : Z -> clause -> list Z -> step.
+
+Definition state := ((zmap cst) * (zmap clause) * Z)%type.
+
+Ltac destate s := destruct s as (p, h) ; destruct p as (cs, cls).
+Inductive status :=
+  | Valid
+  | Invalid
+  | Incomplete : state -> status.
+
+Definition eval_cstmap cs theta :=
+  forall (id : Z) (c : cst),
+    ZMaps.MapsTo id c cs -> eval_cst c theta.
+
+Definition state_csts (s : state) :=
+  match s with
+  | (cs, clauses, hint) => cs
+  end.
+
+Definition eval_clmap clauses theta :=
+  forall id cl, ZMaps.MapsTo id cl clauses -> eval_clause cl theta.
+
+Definition inference_valid (s : state) (cl : clause) :=
+  match s with
+  | (cs, clauses, old) => forall theta,
+      eval_cstmap cs theta -> eval_clause cl theta
+  end.
+
+Definition state_valid (s : state) :=
+  match s with
+  | (cs, clauses, old) => forall (id : Z) (cl : clause),
+      ZMaps.MapsTo id cl clauses -> forall theta,
+        eval_cstmap cs theta -> eval_clause cl theta
+  end.
+  
+Definition clause_map_add (cs : clause_map) (id : Z) (cl : clause) := ZMaps.add id cl cs.
+
+Definition clause_map_del (cs : clause_map) (id : Z) := ZMaps.remove id cs.
+
+
+Lemma clause_map_1 : forall cs cl id theta,
+  eval_clmap cs theta -> eval_clause cl theta -> eval_clmap (clause_map_add cs id cl) theta.
+Proof.
+  unfold eval_clmap, clause_map_add; intros.
+  apply ZMapProperties.F.add_mapsto_iff in H1; destruct H1 as [Heq | Hneq];
+    [ destruct Heq as [Hid Hcl]; now rewrite <- Hcl
+    | destruct Hneq as [Hid Hmap] ; now apply H with (id := id0) ].
+Qed.
+
+Lemma clause_map_2 : forall cs id theta,
+  eval_clmap cs theta -> eval_clmap (clause_map_del cs id) theta.
+Proof.
+  unfold eval_clmap, clause_map_del; intros.
+  apply ZMaps.remove_3 in H0; now apply H with (id := id0).
+Qed.
+
+Definition check_inference (s : state) (cl : clause) :=
+  match s with
+  | (csts, clauses, hint) =>
+    match ZMaps.find hint csts with
+    | None => false
+    | Some cst => check_cst cst cl
+    end
+  end.
+
+(*
+Lemma check_inference_valid : forall (s : state) (cl : clause) (theta : asg),
+  check_inference s cl = true -> eval_cstmap (state_csts s) theta -> eval_clause cl theta.
+Proof.
+  (* Add proof *)
+Qed.
+*)
+
+Definition apply_inference (s : state) (id : Z) (cl : clause) := Invalid.
+Definition apply_resolution (s : state) (id : Z) (cl : clause) (ants : list Z) := Invalid.
+
+Definition set_hint (s : state) (hint : Z) : state:=
+  match s with
+  | (csts, clauses, old) => (csts, clauses, hint)
+  end.
+Lemma set_hint_valid : forall (s : state) (hint : Z),
+  state_valid s -> state_valid (set_hint s hint).
+Proof.
+  unfold state_valid, set_hint; destate s; simpl; intros.
+  now apply H with (id := id).
+Qed.
+
+Definition del_clause (s : state) cid :=
+  match s with
+  | (cs, clauses, hint) => (cs, ZMaps.remove cid clauses, hint)
+  end.
+Lemma del_clause_valid : forall s id, state_valid s -> state_valid (del_clause s id).
+Proof.
+  unfold del_clause, state_valid; destate s; simpl; intros.
+  apply ZMaps.remove_3 in H0.
+  now apply H with (id := id0) (cl := cl) (theta := theta) in H0.
+Qed.
+
+Definition add_clause (s : state) cid cl :=
+  match s with
+  | (cs, clauses, hint) => (cs, ZMaps.add cid cl clauses, hint)
+  end.
+Theorem add_clause_valid : forall (s : state) (id : Z) (cl : clause),
+  state_valid s -> inference_valid s cl -> state_valid (add_clause s id cl).
+Proof.
+  unfold state_valid, inference_valid, add_clause;
+  destate s; simpl; intros.
+  apply ZMapProperties.F.add_mapsto_iff in H1.
+  destruct H1 as [Heq | Hdis].
+  destruct Heq as [Hid Hcl]; rewrite <- Hcl; now apply H0.
+  destruct Hdis as [Hid Hmap].
+  now  apply H with (id := id0) (cl := cl0) (theta := theta).
+Qed.
+  
+Definition apply_step (s : status) (d : step) :=
+  match s with
+  | Valid => Valid
+  | Invalid => Invalid
+  | Incomplete state =>
+    match d with
+    | Intro cid cl => apply_inference state cid cl
+    | Hint cid => Incomplete (set_hint state cid)
+    | Del cid => Incomplete (del_clause state cid)
+    | Resolve cid cl ants => apply_resolution state cid cl ants
+    end
+  end.
+    
