checker/coq/resolution.v
@@ -1,0 +1,27 @@
+(* Resolution of clauses. *)
+Require Import prim.
+Require Lists.List.
+
+(* Actually, we can get away with doing deduplication in a preprocess;
+ * soundness doesn't rely on preserving the proof semantics, just the
+ * _existence_ of a correct proof. *)
+Fixpoint dedup (cl : clause) := 
+  match cl with
+  | nil => nil
+  | cons l cl' =>
+      if List.existsb (lit_eqb l) cl'
+      then
+        (dedup cl')
+      else
+        cons l (dedup cl')
+  end.
+
+(* FIXME: Implement resolvable. *)
+Definition resolvable (cl : clause) (ants : list clause) :=
+  false.
+
+Theorem resolvable_valid : forall cl ants,
+  resolvable cl ants = true -> forall theta, eval_clauses ants theta -> eval_clause cl theta.
+Proof.
+  intros cl ants; unfold resolvable; discriminate.
+Qed.
